add pumping lemmas

Automata/DFA.lean
@@ -1,20 +1,130 @@
 import Mathlib.Tactic
+import Mathlib.Computability.Language
+
+open Computability
 
 structure DFAO (α state out: Type):=
   (transition : α → state → state)
   (start : state)
   (output : state → out)
 
-def DFAO.transFrom (dfao : DFAO α state out) (s : List α) (q : state) : state :=
-  match s with
-    | [] => q
-    | a::as => DFAO.transFrom dfao as (dfao.transition a q)
+variable {α state out : Type}
 
-def DFAO.evalFrom (dfao : DFAO α state out) (s : List α) (q : state) : out :=
-  dfao.output (DFAO.transFrom dfao s q)
+def DFAO.transFrom (dfao : DFAO α state out) (x : List α) (s : state) : state :=
+  match x with
+    | [] => s
+    | a::as => DFAO.transFrom dfao as (dfao.transition a s)
 
-def DFAO.eval (dfao : DFAO α state out) (s : List α) : out :=
-  DFAO.evalFrom dfao s dfao.start
+-- The following theorems and proofs until the pumping lemmas are based on Mathlib's Computability.DFA
+theorem DFAO.transFrom_of_append (dfao: DFAO α state out)(start : state) (x y : List α) :
+    dfao.transFrom (x ++ y) start = dfao.transFrom y (dfao.transFrom x start) := by
+  induction x generalizing start with
+  | nil => rfl
+  | cons a x ih =>
+    simp only [List.append, DFAO.transFrom]
+    specialize ih (dfao.transition a start)
+    simp only [List.append_eq, ih]
+
+theorem DFAO.transFrom_split [Fintype state] {dfao : DFAO α state out} {x : List α} {s t : state} (hlen : Fintype.card state ≤ x.length)
+    (hx : dfao.transFrom x s = t) :
+    ∃ q a b c,
+      x = a ++ b ++ c ∧
+        a.length + b.length ≤ Fintype.card state ∧
+          b ≠ [] ∧ dfao.transFrom a s = q ∧ dfao.transFrom b q = q ∧ dfao.transFrom c q = t := by
+  obtain ⟨n, m, hneq, heq⟩ :=
+    Fintype.exists_ne_map_eq_of_card_lt
+      (fun n : Fin (Fintype.card state + 1) => dfao.transFrom (x.take n) s) (by norm_num)
+  wlog hle : (n : ℕ) ≤ m generalizing n m
+  · exact this m n hneq.symm heq.symm (le_of_not_le hle)
+  have hm : (m : ℕ) ≤ Fintype.card state := Fin.is_le m
+  refine
+    ⟨dfao.transFrom ((x.take m).take n) s, (x.take m).take n, (x.take m).drop n,
+                    x.drop m, ?_, ?_, ?_, by rfl, ?_⟩
+  · rw [List.take_append_drop, List.take_append_drop]
+  · simp only [List.length_drop, List.length_take]
+    rw [min_eq_left (hm.trans hlen), min_eq_left hle, add_tsub_cancel_of_le hle]
+    exact hm
+  · intro h
+    have hlen' := congr_arg List.length h
+    simp only [List.length_drop, List.length, List.length_take] at hlen'
+    rw [min_eq_left, tsub_eq_zero_iff_le] at hlen'
+    · apply hneq
+      apply le_antisymm
+      assumption'
+    exact hm.trans hlen
+  have hq : dfao.transFrom ((x.take m).drop n) (dfao.transFrom ((x.take m).take n) s) =
+      dfao.transFrom ((x.take m).take n) s := by
+    rw [List.take_take, min_eq_left hle, ← transFrom_of_append, heq, ← min_eq_left hle, ←
+      List.take_take, min_eq_left hle, List.take_append_drop]
+  use hq
+  rwa [← hq, ← transFrom_of_append, ← transFrom_of_append, ← List.append_assoc,
+    List.take_append_drop, List.take_append_drop]
+
+theorem DFAO.transFrom_of_pow {dfao : DFAO α state out} {x y : List α} {s : state} (hx : dfao.transFrom x s = s)
+    (hy : y ∈ ({x} : Language α)∗) : dfao.transFrom y s = s := by
+  rw [Language.mem_kstar] at hy
+  rcases hy with ⟨S, rfl, hS⟩
+  induction' S with a S ih
+  · rfl
+  · have ha := hS a (List.mem_cons_self _ _)
+    rw [Set.mem_singleton_iff] at ha
+    rw [List.join, DFAO.transFrom_of_append, ha, hx]
+    apply ih
+    intro z hz
+    exact hS z (List.mem_cons_of_mem a hz)
+
+theorem DFAO.pumping_lemma_trans [Fintype state] {dfao : DFAO α state out} {x : List α} {s t : state} (hx : dfao.transFrom x s = t)(hlen : Fintype.card state ≤ x.length) :
+    ∃ a b c, x = a ++ b ++ c ∧ a.length + b.length ≤ Fintype.card state ∧ b ≠ []
+      ∧ ∀ y ∈ ({a} * {b}∗ * {c} : Language α), dfao.transFrom y s = t := by
+  obtain ⟨q, a, b, c, h, hlen', hne, ha, hb, hc⟩ := dfao.transFrom_split hlen hx
+  use a, b, c
+  constructor
+  . exact h
+  constructor
+  . exact hlen'
+  constructor
+  . exact hne
+  . intro y hy
+    simp [Language.mem_mul] at hy
+    rcases hy with ⟨i, hi, j, hj, k, hk, hy⟩
+    rw[Set.mem_singleton_iff] at hi
+    rw[Set.mem_singleton_iff] at hk
+    rw[← hy, DFAO.transFrom_of_append, hi, ha, DFAO.transFrom_of_append, hk, DFAO.transFrom_of_pow hb]
+    exact hc
+    exact hj
+
+def DFAO.evalFrom (dfao : DFAO α state out) (x : List α) (q : state) : out :=
+  dfao.output (DFAO.transFrom dfao x q)
+
+def DFAO.eval (dfao : DFAO α state out) (x : List α) : out :=
+  DFAO.evalFrom dfao x dfao.start
+
+def DFAO.evalFrom_of_append (dfao : DFAO α state out) (x y : List α) (q : state) :
+  dfao.evalFrom (x ++ y) q = dfao.evalFrom y (dfao.transFrom x q) := by
+  simp[DFAO.evalFrom, DFAO.transFrom_of_append]
+
+def DFAO.pumping_lemma_evalFrom [Fintype state] {dfao : DFAO α state out} {x : List α} {s : state} {o : out} (hx : dfao.evalFrom x s = o)(hlen : Fintype.card state ≤ x.length) :
+    ∃ a b c, x = a ++ b ++ c ∧ a.length + b.length ≤ Fintype.card state ∧ b ≠ []
+      ∧ ∀ y ∈ ({a} * {b}∗ * {c} : Language α), dfao.evalFrom y s = o := by
+  let t := dfao.transFrom x s
+  have hx' : dfao.transFrom x s = t := by rfl
+  obtain ⟨a, b, c, h, hablen, hne, hy⟩ := dfao.pumping_lemma_trans hx' hlen
+  use a, b, c
+  constructor
+  . exact h
+  constructor
+  . exact hablen
+  constructor
+  . exact hne
+  . intro y hy'
+    specialize hy y hy'
+    simp only [evalFrom] at hx
+    simp only [evalFrom, hy, hx]
+
+def DFAO.pumping_lemma_eval [Fintype state] {dfao : DFAO α state out} {x : List α} {o : out} (hx : dfao.eval x = o)(hlen : Fintype.card state ≤ x.length) :
+    ∃ a b c, x = a ++ b ++ c ∧ a.length + b.length ≤ Fintype.card state ∧ b ≠ []
+      ∧ ∀ y ∈ ({a} * {b}∗ * {c} : Language α), dfao.eval y = o := by
+  exact dfao.pumping_lemma_evalFrom hx hlen
 
 -- A DFA is a DFAO where the output is a boolean
 abbrev DFA (α state : Type) := DFAO α state Bool
@@ -39,19 +149,20 @@ def DFAO.toDFA_eval (dfao : DFAO α state out)
     (dfao.toDFA o).eval s = (dfao.eval s == o) := by
   exact DFAO.toDFA_evalFrom dfao o s dfao.start
 
+-- Operations on DFAs: negation, intersection, union
 def DFA.negate (dfa: DFA α state) : DFA α state := {
   transition := dfa.transition
   start := dfa.start
   output := fun x =>  ! dfa.output x
 }
 
-def DFA.product_i (dfa1 : DFA α state1) (dfa2 : DFA α state2) : DFA (α ) (state1 × state2) := {
+def DFA.intersection (dfa1 : DFA α state1) (dfa2 : DFA α state2) : DFA (α ) (state1 × state2) := {
   transition := fun a q => ⟨dfa1.transition a q.1, dfa2.transition a q.2⟩,
   start := (dfa1.start, dfa2.start),
   output := fun (q1, q2) => dfa1.output q1 && dfa2.output q2
 }
 
-def DFA.product_u  (dfa1 : DFA α state1) (dfa2 : DFA α state2) : DFA (α) (state1 × state2) := {
+def DFA.union  (dfa1 : DFA α state1) (dfa2 : DFA α state2) : DFA (α) (state1 × state2) := {
   transition := fun a q => ⟨dfa1.transition a q.1, dfa2.transition a q.2⟩,
   start := (dfa1.start, dfa2.start),
   output := fun (q1, q2) => dfa1.output q1 || dfa2.output q2
@@ -78,44 +189,44 @@ theorem DFA.negate_eval (dfa : DFA α state) (s : List α) :
   (dfa.negate).eval s = ! dfa.eval s := by
   exact DFA.negate_evalFrom dfa s dfa.start
 
-theorem DFA.product_i_output (dfa1 : DFA α state1) (dfa2 : DFA α state2) (q1 : state1) (q2 : state2) :
-  (dfa1.product_i dfa2).output (q1, q2) = (dfa1.output q1 && dfa2.output q2) := by rfl
+theorem DFA.intersection_output (dfa1 : DFA α state1) (dfa2 : DFA α state2) (q1 : state1) (q2 : state2) :
+  (dfa1.intersection dfa2).output (q1, q2) = (dfa1.output q1 && dfa2.output q2) := by rfl
 
-theorem DFA.product_i_transition (dfa1 : DFA α state1) (dfa2 : DFA α state2) :
-  (dfa1.product_i dfa2).transition = fun a q => ⟨dfa1.transition a q.1, dfa2.transition a q.2⟩ := by rfl
+theorem DFA.intersection_transition (dfa1 : DFA α state1) (dfa2 : DFA α state2) :
+  (dfa1.intersection dfa2).transition = fun a q => ⟨dfa1.transition a q.1, dfa2.transition a q.2⟩ := by rfl
 
-theorem DFA.product_i_transFrom (dfa1 : DFA α state1) (dfa2 : DFA α state2) (s : List α) (q1 : state1) (q2 : state2) :
-  (dfa1.product_i dfa2).transFrom s (q1, q2) = (dfa1.transFrom s q1, dfa2.transFrom s q2) := by
+theorem DFA.intersection_transFrom (dfa1 : DFA α state1) (dfa2 : DFA α state2) (s : List α) (q1 : state1) (q2 : state2) :
+  (dfa1.intersection dfa2).transFrom s (q1, q2) = (dfa1.transFrom s q1, dfa2.transFrom s q2) := by
   induction s generalizing q1 q2
   case nil => rfl
   case cons a s ih =>
-    simp [DFAO.transFrom, DFA.product_i_transition, ih]
+    simp [DFAO.transFrom, DFA.intersection_transition, ih]
 
-theorem DFA.product_i_evalFrom (dfa1 : DFA α state1) (dfa2 : DFA α state2) (s : List α) (q1 : state1) (q2 : state2) :
-  (dfa1.product_i dfa2).evalFrom s (q1, q2) = (dfa1.evalFrom s q1 && dfa2.evalFrom s q2) := by
-  simp[DFAO.evalFrom, DFA.product_i_transFrom, DFA.product_i_output]
+theorem DFA.intersection_evalFrom (dfa1 : DFA α state1) (dfa2 : DFA α state2) (s : List α) (q1 : state1) (q2 : state2) :
+  (dfa1.intersection dfa2).evalFrom s (q1, q2) = (dfa1.evalFrom s q1 && dfa2.evalFrom s q2) := by
+  simp[DFAO.evalFrom, DFA.intersection_transFrom, DFA.intersection_output]
 
-theorem DFA.product_i_eval (dfa1 : DFA α state1) (dfa2 : DFA α state2)
-  (s : List α) : (dfa1.product_i dfa2).eval s = (dfa1.eval s && dfa2.eval s) := by
-  exact DFA.product_i_evalFrom dfa1 dfa2 s dfa1.start dfa2.start
+theorem DFA.intersection_eval (dfa1 : DFA α state1) (dfa2 : DFA α state2)
+  (s : List α) : (dfa1.intersection dfa2).eval s = (dfa1.eval s && dfa2.eval s) := by
+  exact DFA.intersection_evalFrom dfa1 dfa2 s dfa1.start dfa2.start
 
-theorem DFA.product_u_output (dfa1 : DFA α state1) (dfa2 : DFA α state2) (q1 : state1) (q2 : state2) :
-  (dfa1.product_u dfa2).output (q1, q2) = (dfa1.output q1 || dfa2.output q2) := by rfl
+theorem DFA.union_output (dfa1 : DFA α state1) (dfa2 : DFA α state2) (q1 : state1) (q2 : state2) :
+  (dfa1.union dfa2).output (q1, q2) = (dfa1.output q1 || dfa2.output q2) := by rfl
 
-theorem DFA.product_u_transition (dfa1 : DFA α state1) (dfa2 : DFA α state2) :
-  (dfa1.product_u dfa2).transition = fun a q => ⟨dfa1.transition a q.1, dfa2.transition a q.2⟩ := by rfl
+theorem DFA.union_transition (dfa1 : DFA α state1) (dfa2 : DFA α state2) :
+  (dfa1.union dfa2).transition = fun a q => ⟨dfa1.transition a q.1, dfa2.transition a q.2⟩ := by rfl
 
-theorem DFA.product_u_transFrom (dfa1 : DFA α state1) (dfa2 : DFA α state2) (s : List α) (q1 : state1) (q2 : state2) :
-  (dfa1.product_u dfa2).transFrom s (q1, q2) = (dfa1.transFrom s q1, dfa2.transFrom s q2) := by
+theorem DFA.union_transFrom (dfa1 : DFA α state1) (dfa2 : DFA α state2) (s : List α) (q1 : state1) (q2 : state2) :
+  (dfa1.union dfa2).transFrom s (q1, q2) = (dfa1.transFrom s q1, dfa2.transFrom s q2) := by
   induction s generalizing q1 q2
   case nil => rfl
   case cons a s ih =>
-    simp [DFAO.transFrom, DFA.product_u_transition, ih]
+    simp [DFAO.transFrom, DFA.union_transition, ih]
 
-theorem DFA.product_u_evalFrom (dfa1 : DFA α state1) (dfa2 : DFA α state2) (s : List α) (q1 : state1) (q2 : state2) :
-  (dfa1.product_u dfa2).evalFrom s (q1, q2) = (dfa1.evalFrom s q1 || dfa2.evalFrom s q2) := by
-  simp[DFAO.evalFrom, DFA.product_u_transFrom, DFA.product_u_output]
+theorem DFA.union_evalFrom (dfa1 : DFA α state1) (dfa2 : DFA α state2) (s : List α) (q1 : state1) (q2 : state2) :
+  (dfa1.union dfa2).evalFrom s (q1, q2) = (dfa1.evalFrom s q1 || dfa2.evalFrom s q2) := by
+  simp[DFAO.evalFrom, DFA.union_transFrom, DFA.union_output]
 
-theorem DFA.product_u_eval (dfa1 : DFA α state1) (dfa2 : DFA α state2)
-  (s : List α) : (dfa1.product_u dfa2).eval s = (dfa1.eval s || dfa2.eval s) := by
-  exact DFA.product_u_evalFrom dfa1 dfa2 s dfa1.start dfa2.start
+theorem DFA.union_eval (dfa1 : DFA α state1) (dfa2 : DFA α state2)
+  (s : List α) : (dfa1.union dfa2).eval s = (dfa1.eval s || dfa2.eval s) := by
+  exact DFA.union_evalFrom dfa1 dfa2 s dfa1.start dfa2.start
