Automata/NFA.lean
@@ -3,6 +3,8 @@ import Mathlib.Data.List.Basic
 import Automata.DFA
 import Mathlib.Data.FinEnum
 
+open Computability
+
 structure NFA (α state : Type) :=
   (transition : α → state → List state)
   (start : List state)
@@ -27,23 +29,23 @@ def NFA.toDFA (nfa : NFA α state) [BEq state] : DFA α (List state) where
 theorem NFA.toDFA_transition (nfa : NFA α state) (a : α) (qs : List state) [BEq state]:
   (nfa.toDFA).transition a qs = NFA.transList nfa a qs := by rfl
 
-theorem NFA.toDFA_evalFrom (nfa : NFA α state) (s : List α) (qs: List state) [BEq state]:
-  (nfa.toDFA).evalFrom s qs = nfa.evalFrom s qs := by
-  induction s generalizing qs
+theorem NFA.toDFA_evalFrom (nfa : NFA α state) (x : List α) (qs: List state) [BEq state]:
+  (nfa.toDFA).evalFrom x qs = nfa.evalFrom x qs := by
+  induction x generalizing qs
   case nil =>
     simp only [NFA.evalFrom, DFAO.evalFrom, DFAO.transFrom, NFA.toDFA]
-  case cons x xs ih =>
+  case cons y ys ih =>
     simp only [NFA.evalFrom, DFAO.evalFrom, NFA.toDFA_transition]
-    exact ih (nfa.transList x qs)
+    exact ih (nfa.transList y qs)
 
 theorem NFA.toDFA_eval (nfa : NFA α state) (s : List α) [BEq state]
   : (nfa.toDFA).eval s = nfa.eval s := NFA.toDFA_evalFrom nfa s nfa.start
 
-
-/- USELESS CODE
-def project' (dfa : DFA (β × α) state) [BEq state] [FinEnum β] : NFA α state := {
-  transition := fun a q => (List.map (fun (x : β) => dfa.transition (x, a) q) (FinEnum.toList β))
-  start := [dfa.start]
-  output := dfa.output
-}
+/- TODO
+theorem NFA.pumping_lemma_evalFrom [Fintype state] [BEq state] {nfa : NFA α state} {x : List α} {qs : List state}(hx : nfa.evalFrom x qs)(hlen : Fintype.card state ≤ x.length) :
+    ∃ a b c, x = a ++ b ++ c ∧ a.length + b.length ≤ Fintype.card state ∧ b ≠ []
+      ∧ ∀ y ∈ ({a} * {b}∗ * {c} : Language α), nfa.evalFrom y qs := by
+  rw [← toDFA_evalFrom] at hx
+  exact nfa.toDFA.pumping_lemma_evalFrom hx hlen
+  done
 -/
